src/impl/TLS13.KeySchedule.fst
@@ -5,16 +5,12 @@ module TLS13.KeySchedule
 open Pulse.Lib.Pervasives
 open Pulse.Lib.Array.PtsTo
 
-module A = Pulse.Lib.Array.PtsTo
 module B = TLS13.Bytes
 module Crypto = TLS13.Crypto
 module K = TLS13.Keys
 module Seq = FStar.Seq
 module SZ = FStar.SizeT
 module U8 = FStar.UInt8
-
-inline_for_extraction
-let zero_u8 : U8.t = U8.uint_to_t 0
 
 noextract
 let label_derived_seq : B.bytes = K.label_derived
@@ -35,16 +31,16 @@ let label_iv_seq : B.bytes = K.label_iv
 
 inline_for_extraction
 fn write_label_derived (lbl: array U8.t)
-  requires pts_to lbl (Seq.create 7 zero_u8)
+  requires pts_to lbl (Seq.create 7 0uy)
   ensures pts_to lbl label_derived_seq
 {
-  lbl.(0sz) <- U8.uint_to_t 0x64;
-  lbl.(1sz) <- U8.uint_to_t 0x65;
-  lbl.(2sz) <- U8.uint_to_t 0x72;
-  lbl.(3sz) <- U8.uint_to_t 0x69;
-  lbl.(4sz) <- U8.uint_to_t 0x76;
-  lbl.(5sz) <- U8.uint_to_t 0x65;
-  lbl.(6sz) <- U8.uint_to_t 0x64;
+  lbl.(0sz) <- 0x64uy;
+  lbl.(1sz) <- 0x65uy;
+  lbl.(2sz) <- 0x72uy;
+  lbl.(3sz) <- 0x69uy;
+  lbl.(4sz) <- 0x76uy;
+  lbl.(5sz) <- 0x65uy;
+  lbl.(6sz) <- 0x64uy;
   with s. assert (pts_to lbl s);
   assert_norm (s == label_derived_seq);
   assert (pure (s == label_derived_seq));
@@ -52,21 +48,21 @@ fn write_label_derived (lbl: array U8.t)
 
 inline_for_extraction
 fn write_label_c_hs_traffic (lbl: array U8.t)
-  requires pts_to lbl (Seq.create 12 zero_u8)
+  requires pts_to lbl (Seq.create 12 0uy)
   ensures pts_to lbl label_c_hs_traffic_seq
 {
-  lbl.(0sz) <- U8.uint_to_t 0x63;
-  lbl.(1sz) <- U8.uint_to_t 0x20;
-  lbl.(2sz) <- U8.uint_to_t 0x68;
-  lbl.(3sz) <- U8.uint_to_t 0x73;
-  lbl.(4sz) <- U8.uint_to_t 0x20;
-  lbl.(5sz) <- U8.uint_to_t 0x74;
-  lbl.(6sz) <- U8.uint_to_t 0x72;
-  lbl.(7sz) <- U8.uint_to_t 0x61;
-  lbl.(8sz) <- U8.uint_to_t 0x66;
-  lbl.(9sz) <- U8.uint_to_t 0x66;
-  lbl.(10sz) <- U8.uint_to_t 0x69;
-  lbl.(11sz) <- U8.uint_to_t 0x63;
+  lbl.(0sz) <- 0x63uy;
+  lbl.(1sz) <- 0x20uy;
+  lbl.(2sz) <- 0x68uy;
+  lbl.(3sz) <- 0x73uy;
+  lbl.(4sz) <- 0x20uy;
+  lbl.(5sz) <- 0x74uy;
+  lbl.(6sz) <- 0x72uy;
+  lbl.(7sz) <- 0x61uy;
+  lbl.(8sz) <- 0x66uy;
+  lbl.(9sz) <- 0x66uy;
+  lbl.(10sz) <- 0x69uy;
+  lbl.(11sz) <- 0x63uy;
   with s. assert (pts_to lbl s);
   assert_norm (s == label_c_hs_traffic_seq);
   assert (pure (s == label_c_hs_traffic_seq));
@@ -74,21 +70,21 @@ fn write_label_c_hs_traffic (lbl: array U8.t)
 
 inline_for_extraction
 fn write_label_s_hs_traffic (lbl: array U8.t)
-  requires pts_to lbl (Seq.create 12 zero_u8)
+  requires pts_to lbl (Seq.create 12 0uy)
   ensures pts_to lbl label_s_hs_traffic_seq
 {
-  lbl.(0sz) <- U8.uint_to_t 0x73;
-  lbl.(1sz) <- U8.uint_to_t 0x20;
-  lbl.(2sz) <- U8.uint_to_t 0x68;
-  lbl.(3sz) <- U8.uint_to_t 0x73;
-  lbl.(4sz) <- U8.uint_to_t 0x20;
-  lbl.(5sz) <- U8.uint_to_t 0x74;
-  lbl.(6sz) <- U8.uint_to_t 0x72;
-  lbl.(7sz) <- U8.uint_to_t 0x61;
-  lbl.(8sz) <- U8.uint_to_t 0x66;
-  lbl.(9sz) <- U8.uint_to_t 0x66;
-  lbl.(10sz) <- U8.uint_to_t 0x69;
-  lbl.(11sz) <- U8.uint_to_t 0x63;
+  lbl.(0sz) <- 0x73uy;
+  lbl.(1sz) <- 0x20uy;
+  lbl.(2sz) <- 0x68uy;
+  lbl.(3sz) <- 0x73uy;
+  lbl.(4sz) <- 0x20uy;
+  lbl.(5sz) <- 0x74uy;
+  lbl.(6sz) <- 0x72uy;
+  lbl.(7sz) <- 0x61uy;
+  lbl.(8sz) <- 0x66uy;
+  lbl.(9sz) <- 0x66uy;
+  lbl.(10sz) <- 0x69uy;
+  lbl.(11sz) <- 0x63uy;
   with s. assert (pts_to lbl s);
   assert_norm (s == label_s_hs_traffic_seq);
   assert (pure (s == label_s_hs_traffic_seq));
@@ -96,21 +92,21 @@ fn write_label_s_hs_traffic (lbl: array U8.t)
 
 inline_for_extraction
 fn write_label_c_ap_traffic (lbl: array U8.t)
-  requires pts_to lbl (Seq.create 12 zero_u8)
+  requires pts_to lbl (Seq.create 12 0uy)
   ensures pts_to lbl label_c_ap_traffic_seq
 {
-  lbl.(0sz) <- U8.uint_to_t 0x63;
-  lbl.(1sz) <- U8.uint_to_t 0x20;
-  lbl.(2sz) <- U8.uint_to_t 0x61;
-  lbl.(3sz) <- U8.uint_to_t 0x70;
-  lbl.(4sz) <- U8.uint_to_t 0x20;
-  lbl.(5sz) <- U8.uint_to_t 0x74;
-  lbl.(6sz) <- U8.uint_to_t 0x72;
-  lbl.(7sz) <- U8.uint_to_t 0x61;
-  lbl.(8sz) <- U8.uint_to_t 0x66;
-  lbl.(9sz) <- U8.uint_to_t 0x66;
-  lbl.(10sz) <- U8.uint_to_t 0x69;
-  lbl.(11sz) <- U8.uint_to_t 0x63;
+  lbl.(0sz) <- 0x63uy;
+  lbl.(1sz) <- 0x20uy;
+  lbl.(2sz) <- 0x61uy;
+  lbl.(3sz) <- 0x70uy;
+  lbl.(4sz) <- 0x20uy;
+  lbl.(5sz) <- 0x74uy;
+  lbl.(6sz) <- 0x72uy;
+  lbl.(7sz) <- 0x61uy;
+  lbl.(8sz) <- 0x66uy;
+  lbl.(9sz) <- 0x66uy;
+  lbl.(10sz) <- 0x69uy;
+  lbl.(11sz) <- 0x63uy;
   with s. assert (pts_to lbl s);
   assert_norm (s == label_c_ap_traffic_seq);
   assert (pure (s == label_c_ap_traffic_seq));
@@ -118,21 +114,21 @@ fn write_label_c_ap_traffic (lbl: array U8.t)
 
 inline_for_extraction
 fn write_label_s_ap_traffic (lbl: array U8.t)
-  requires pts_to lbl (Seq.create 12 zero_u8)
+  requires pts_to lbl (Seq.create 12 0uy)
   ensures pts_to lbl label_s_ap_traffic_seq
 {
-  lbl.(0sz) <- U8.uint_to_t 0x73;
-  lbl.(1sz) <- U8.uint_to_t 0x20;
-  lbl.(2sz) <- U8.uint_to_t 0x61;
-  lbl.(3sz) <- U8.uint_to_t 0x70;
-  lbl.(4sz) <- U8.uint_to_t 0x20;
-  lbl.(5sz) <- U8.uint_to_t 0x74;
-  lbl.(6sz) <- U8.uint_to_t 0x72;
-  lbl.(7sz) <- U8.uint_to_t 0x61;
-  lbl.(8sz) <- U8.uint_to_t 0x66;
-  lbl.(9sz) <- U8.uint_to_t 0x66;
-  lbl.(10sz) <- U8.uint_to_t 0x69;
-  lbl.(11sz) <- U8.uint_to_t 0x63;
+  lbl.(0sz) <- 0x73uy;
+  lbl.(1sz) <- 0x20uy;
+  lbl.(2sz) <- 0x61uy;
+  lbl.(3sz) <- 0x70uy;
+  lbl.(4sz) <- 0x20uy;
+  lbl.(5sz) <- 0x74uy;
+  lbl.(6sz) <- 0x72uy;
+  lbl.(7sz) <- 0x61uy;
+  lbl.(8sz) <- 0x66uy;
+  lbl.(9sz) <- 0x66uy;
+  lbl.(10sz) <- 0x69uy;
+  lbl.(11sz) <- 0x63uy;
   with s. assert (pts_to lbl s);
   assert_norm (s == label_s_ap_traffic_seq);
   assert (pure (s == label_s_ap_traffic_seq));
@@ -140,17 +136,17 @@ fn write_label_s_ap_traffic (lbl: array U8.t)
 
 inline_for_extraction
 fn write_label_finished (lbl: array U8.t)
-  requires pts_to lbl (Seq.create 8 zero_u8)
+  requires pts_to lbl (Seq.create 8 0uy)
   ensures pts_to lbl label_finished_seq
 {
-  lbl.(0sz) <- U8.uint_to_t 0x66;
-  lbl.(1sz) <- U8.uint_to_t 0x69;
-  lbl.(2sz) <- U8.uint_to_t 0x6e;
-  lbl.(3sz) <- U8.uint_to_t 0x69;
-  lbl.(4sz) <- U8.uint_to_t 0x73;
-  lbl.(5sz) <- U8.uint_to_t 0x68;
-  lbl.(6sz) <- U8.uint_to_t 0x65;
-  lbl.(7sz) <- U8.uint_to_t 0x64;
+  lbl.(0sz) <- 0x66uy;
+  lbl.(1sz) <- 0x69uy;
+  lbl.(2sz) <- 0x6euy;
+  lbl.(3sz) <- 0x69uy;
+  lbl.(4sz) <- 0x73uy;
+  lbl.(5sz) <- 0x68uy;
+  lbl.(6sz) <- 0x65uy;
+  lbl.(7sz) <- 0x64uy;
   with s. assert (pts_to lbl s);
   assert_norm (s == label_finished_seq);
   assert (pure (s == label_finished_seq));
@@ -158,12 +154,12 @@ fn write_label_finished (lbl: array U8.t)
 
 inline_for_extraction
 fn write_label_key (lbl: array U8.t)
-  requires pts_to lbl (Seq.create 3 zero_u8)
+  requires pts_to lbl (Seq.create 3 0uy)
   ensures pts_to lbl label_key_seq
 {
-  lbl.(0sz) <- U8.uint_to_t 0x6b;
-  lbl.(1sz) <- U8.uint_to_t 0x65;
-  lbl.(2sz) <- U8.uint_to_t 0x79;
+  lbl.(0sz) <- 0x6buy;
+  lbl.(1sz) <- 0x65uy;
+  lbl.(2sz) <- 0x79uy;
   with s. assert (pts_to lbl s);
   assert_norm (s == label_key_seq);
   assert (pure (s == label_key_seq));
@@ -171,16 +167,17 @@ fn write_label_key (lbl: array U8.t)
 
 inline_for_extraction
 fn write_label_iv (lbl: array U8.t)
-  requires pts_to lbl (Seq.create 2 zero_u8)
+  requires pts_to lbl (Seq.create 2 0uy)
   ensures pts_to lbl label_iv_seq
 {
-  lbl.(0sz) <- U8.uint_to_t 0x69;
-  lbl.(1sz) <- U8.uint_to_t 0x76;
+  lbl.(0sz) <- 0x69uy;
+  lbl.(1sz) <- 0x76uy;
   with s. assert (pts_to lbl s);
   assert_norm (s == label_iv_seq);
   assert (pure (s == label_iv_seq));
 }
 
+inline_for_extraction
 fn derived_secret
   (secret: array U8.t)
   (out: array U8.t)
@@ -190,15 +187,12 @@ fn derived_secret
   ensures pts_to secret 'secret_bytes **
           pts_to out (K.derived_secret (Ghost.reveal 'secret_bytes))
 {
-  let empty_hash = A.alloc zero_u8 32sz;
+  let mut empty_hash = [| 0uy; 32sz |];
   Crypto.sha256_empty empty_hash;
 
-  let lbl = A.alloc zero_u8 7sz;
+  let mut lbl = [| 0uy; 7sz |];
   write_label_derived lbl;
   Crypto.hkdf_expand_label secret lbl 7sz empty_hash 32sz out 32sz;
-
-  A.free lbl;
-  A.free empty_hash;
 }
 
 fn handshake_secret
@@ -216,10 +210,9 @@ fn handshake_secret
           pts_to shared 'shared_bytes **
           pts_to out (K.handshake_secret (Ghost.reveal 'early_bytes) (Ghost.reveal 'shared_bytes))
 {
-  let derived = A.alloc zero_u8 32sz;
+  let mut derived = [| 0uy; 32sz |];
   derived_secret early derived;
   Crypto.hkdf_extract derived 32sz shared shared_len out;
-  A.free derived;
 }
 
 fn master_secret
@@ -231,12 +224,10 @@ fn master_secret
   ensures pts_to handshake 'handshake_bytes **
           pts_to out (K.master_secret (Ghost.reveal 'handshake_bytes))
 {
-  let derived = A.alloc zero_u8 32sz;
+  let mut derived = [| 0uy; 32sz |];
   derived_secret handshake derived;
-  let zero = A.alloc zero_u8 32sz;
+  let mut zero = [| 0uy; 32sz |];
   Crypto.hkdf_extract derived 32sz zero 32sz out;
-  A.free zero;
-  A.free derived;
 }
 
 fn client_handshake_traffic_secret
@@ -255,10 +246,9 @@ fn client_handshake_traffic_secret
                         (Ghost.reveal 'handshake_bytes)
                         (Ghost.reveal 'hash_bytes))
 {
-  let lbl = A.alloc zero_u8 12sz;
+  let mut lbl = [| 0uy; 12sz |];
   write_label_c_hs_traffic lbl;
   Crypto.hkdf_expand_label handshake lbl 12sz transcript_hash 32sz out 32sz;
-  A.free lbl;
 }
 
 fn server_handshake_traffic_secret
@@ -277,10 +267,9 @@ fn server_handshake_traffic_secret
                         (Ghost.reveal 'handshake_bytes)
                         (Ghost.reveal 'hash_bytes))
 {
-  let lbl = A.alloc zero_u8 12sz;
+  let mut lbl = [| 0uy; 12sz |];
   write_label_s_hs_traffic lbl;
   Crypto.hkdf_expand_label handshake lbl 12sz transcript_hash 32sz out 32sz;
-  A.free lbl;
 }
 
 fn client_application_traffic_secret
@@ -299,10 +288,9 @@ fn client_application_traffic_secret
                         (Ghost.reveal 'master_bytes)
                         (Ghost.reveal 'hash_bytes))
 {
-  let lbl = A.alloc zero_u8 12sz;
+  let mut lbl = [| 0uy; 12sz |];
   write_label_c_ap_traffic lbl;
   Crypto.hkdf_expand_label master lbl 12sz transcript_hash 32sz out 32sz;
-  A.free lbl;
 }
 
 fn server_application_traffic_secret
@@ -321,10 +309,9 @@ fn server_application_traffic_secret
                         (Ghost.reveal 'master_bytes)
                         (Ghost.reveal 'hash_bytes))
 {
-  let lbl = A.alloc zero_u8 12sz;
+  let mut lbl = [| 0uy; 12sz |];
   write_label_s_ap_traffic lbl;
   Crypto.hkdf_expand_label master lbl 12sz transcript_hash 32sz out 32sz;
-  A.free lbl;
 }
 
 fn finished_verify_data
@@ -343,13 +330,11 @@ fn finished_verify_data
                        (Ghost.reveal 'base_key_bytes)
                        (Ghost.reveal 'hash_bytes))
 {
-  let lbl = A.alloc zero_u8 8sz;
+  let mut lbl = [| 0uy; 8sz |];
   write_label_finished lbl;
-  let finished_key = A.alloc zero_u8 32sz;
+  let mut finished_key = [| 0uy; 32sz |];
   Crypto.hkdf_expand_label_empty_context base_key lbl 8sz finished_key 32sz;
   Crypto.hmac_sha256 finished_key 32sz transcript_hash 32sz out;
-  A.free finished_key;
-  A.free lbl;
 }
 
 fn derive_traffic_key
@@ -361,10 +346,9 @@ fn derive_traffic_key
   ensures pts_to traffic_secret 'secret_bytes **
           pts_to out (K.derive_aead_key (Ghost.reveal 'secret_bytes))
 {
-  let lbl = A.alloc zero_u8 3sz;
+  let mut lbl = [| 0uy; 3sz |];
   write_label_key lbl;
   Crypto.hkdf_expand_label_empty_context traffic_secret lbl 3sz out 32sz;
-  A.free lbl;
 }
 
 fn derive_traffic_iv
@@ -376,8 +360,7 @@ fn derive_traffic_iv
   ensures pts_to traffic_secret 'secret_bytes **
           pts_to out (K.derive_aead_iv (Ghost.reveal 'secret_bytes))
 {
-  let lbl = A.alloc zero_u8 2sz;
+  let mut lbl = [| 0uy; 2sz |];
   write_label_iv lbl;
   Crypto.hkdf_expand_label_empty_context traffic_secret lbl 2sz out 12sz;
-  A.free lbl;
 }
