src/impl/TLS13.Extract.Smoke.fst
@@ -4,10 +4,10 @@ module U8 = FStar.UInt8
 module U16 = FStar.UInt16
 
 let tls13_version_major (_:unit) : U8.t =
-  U8.uint_to_t 3
+  3uy
 
 let tls13_version_minor (_:unit) : U8.t =
-  U8.uint_to_t 4
+  4uy
 
 let tls13_chacha20_poly1305_sha256 (_:unit) : U16.t =
-  U16.uint_to_t 0x1303
+  0x1303us
