src/spec/TLS13.Bytes.fst
@@ -1,14 +1,12 @@
 module TLS13.Bytes
 
 module Seq = FStar.Seq
-module U8 = FStar.UInt8
-
-type byte = U8.t
+type byte = FStar.UInt8.t
 type bytes = Seq.seq byte
 
 let length (b:bytes) : nat = Seq.length b
 
-let zero : byte = U8.uint_to_t 0
+let zero : byte = 0uy
 
 let empty : bytes = Seq.create 0 zero
 
